Lean/Geo/KGon/Var.lean
@@ -9,34 +9,38 @@ namespace Geo
 inductive Var (n : Nat) where
   | sigma  (a b c : Fin n)
   | inside (x a b c : Fin n)
-  | hole   (a b c : Fin n)
+  | hole₀  (a : Fin (n+1)) (b c : Fin n)
   | cap    (a c d : Fin n)
   | cup    (a c d : Fin n)
   | capF   (a d e : Fin n)
   deriving DecidableEq
 
+instance : Inhabited (Var (n+1)) := ⟨.sigma 0 0 0⟩
+
+def Var.hole (a b c : Fin n) := Var.hole₀ a.succ b c
+
 instance : Repr (Var n) where
   reprPrec
-  | .sigma a b c, _ => f!"σ {a} {b} {c}"
-  | .inside x a b c, _ => f!"inside {x} {a} {b} {c}"
-  | .hole a b c, _ => f!"hole {a} {b} {c}"
-  | .cap a b c, _ => f!"cap {a} {b} {c}"
-  | .cup a b c, _ => f!"cup {a} {b} {c}"
-  | .capF a b c, _ => f!"capF {a} {b} {c}"
+  | .sigma a b c, _ => f!"σ {a.succ} {b.succ} {c.succ}"
+  | .inside x a b c, _ => f!"inside {x.succ} {a.succ} {b.succ} {c.succ}"
+  | .hole₀ a b c, _ => f!"hole {a} {b.succ} {c.succ}"
+  | .cap a b c, _ => f!"cap {a.succ} {b.succ} {c.succ}"
+  | .cup a b c, _ => f!"cup {a.succ} {b.succ} {c.succ}"
+  | .capF a b c, _ => f!"capF {a.succ} {b.succ} {c.succ}"
 
 -- TODO: make a deriving instance for `LinearOrder`
 instance : LinearOrder (Var n) :=
   LinearOrder.lift'
     (β := (Fin n ×ₗ Fin n ×ₗ Fin n ⊕ₗ
            Fin n ×ₗ Fin n ×ₗ Fin n ×ₗ Fin n ⊕ₗ
-           Fin n ×ₗ Fin n ×ₗ Fin n) ⊕ₗ
+           Fin (n+1) ×ₗ Fin n ×ₗ Fin n) ⊕ₗ
            Fin n ×ₗ Fin n ×ₗ Fin n ⊕ₗ
            Fin n ×ₗ Fin n ×ₗ Fin n ⊕ₗ
            Fin n ×ₗ Fin n ×ₗ Fin n)
     (fun
       | .sigma a b c => .inlₗ <| .inlₗ (a, b, c)
       | .inside x a b c => .inlₗ <| .inrₗ <| .inlₗ (x, a, b, c)
-      | .hole a b c => .inlₗ <| .inrₗ <| .inrₗ (a, b, c)
+      | .hole₀ a b c => .inlₗ <| .inrₗ <| .inrₗ (a, b, c)
       | .cap a c d => .inrₗ <| .inlₗ (a, c, d)
       | .capF a d e => .inrₗ <| .inrₗ <| .inlₗ (a, d, e)
       | .cup a c d => .inrₗ <| .inrₗ <| .inrₗ (a, c, d))
@@ -45,7 +49,7 @@ instance : LinearOrder (Var n) :=
 def Var.toCode : Var n → String
   | .sigma a b c => s!"0 0 {a} {b} {c}"
   | .inside x a b c => s!"1 {x} {a} {b} {c}"
-  | .hole a b c => s!"2 0 {a} {b} {c}"
+  | .hole₀ a b c => s!"2 0 {a} {b} {c}"
   | .cap a b c => s!"3 0 {a} {b} {c}"
   | .cup a b c => s!"4 0 {a} {b} {c}"
   | .capF a b c => s!"5 0 {a} {b} {c}"
