Lean/Geo/Naive/Assn.lean
@@ -1,0 +1,101 @@
+import Geo.Definitions.CanonicalPoints
+import Geo.Definitions.PtInTriangle
+import Geo.Definitions.Structures
+import Geo.Definitions.OrientationProperties
+import Geo.Orientations
+import Geo.Naive.Encoding
+import Geo.KGon.Assn
+
+namespace Geo.CanonicalPoints
+open List Classical Point
+attribute [-simp] getElem_fin
+
+def isKHole1 (w : CanonicalPoints) (s : Finset (Fin w.length)) (b c : Fin w.length) :=
+  ∀ᵉ (a ∈ s), a < b → σIsEmptyTriangleFor w[a] w[b] w[c] w.toFinset
+
+def isKHole2 (w : CanonicalPoints) (s : Finset (Fin w.length)) (c : Fin w.length) :=
+  ∀ᵉ (b ∈ s), b < c → isKHole1 w s b c
+
+def isKHole (w : CanonicalPoints) (s : Finset (Fin w.length)) := ∀ᵉ (c ∈ s), isKHole2 w s c
+
+theorem satisfies_noKHoleClausesCore {w : CanonicalPoints}
+    {k i G1 G2} (T : Finset (Fin w.length)) (hh : isKHole w T)
+    (hT1 : ∀ x ∈ T, x.1 ≤ i)
+    (hs : ∀ s, s.card = k → (∀ x ∈ s, i < x.1) → ¬isKHole w (T ∪ s))
+    (hG1 : ∀ b c, i ≤ b.1 → b < c → (G1 b c).eval w.toPropAssn → isKHole1 w T b.succ c.succ)
+    (hG2 : ∀ c, i ≤ c.1 → (G2 c).eval w.toPropAssn → isKHole2 w T c.succ) :
+    (noKHoleClausesCore w.rlen k i G1 G2).eval w.toPropAssn := by
+  rw [noKHoleClausesCore]; split_ifs with k0
+  · simp; intro hi
+    constructor
+    · intro h1
+      let i' : Fin w.rlen := ⟨i, hi⟩
+      refine satisfies_noKHoleClausesCore (insert i'.succ T) ?_ ?_ (fun s sz hs' => ?_) ?_ ?_
+      · intro c hc b hb bc a ha ab
+        simp (config := {zeta := false}) at ha hb hc
+        have : c ≤ i'.succ := by obtain rfl | hc := hc <;> [rfl; exact Nat.le_succ_of_le (hT1 _ hc)]
+        have ha := ha.resolve_left <| ne_of_lt <| lt_of_lt_of_le (ab.trans bc) this
+        have hb' := lt_of_lt_of_le bc this
+        have hb := hb.resolve_left <| ne_of_lt hb'
+        obtain rfl | hc := hc
+        · exact hG2 i' le_rfl h1 b hb hb' a ha ab
+        · exact hh _ hc _ hb bc _ ha ab
+      · simp; exact fun x hx => Nat.le_succ_of_le (hT1 _ hx)
+      · rw [Finset.insert_union, ← Finset.union_insert]
+        apply hs
+        · rw [Finset.card_insert_of_not_mem, sz, Nat.sub_add_cancel k0]
+          exact fun h => lt_irrefl _ (hs' _ h)
+        · simp; exact fun x hx => Nat.le_of_lt (hs' _ hx)
+      · simp (config := {zeta := false}); intro b c ib bc h1 h2 a ha ab
+        obtain rfl | ha := Finset.mem_insert.1 ha
+        · exact h1
+        · exact hG1 b c (Nat.le_of_lt ib) bc h2 _ ha ab
+      · simp (config := {zeta := false}); intro c ic h1 h2 b hb bc a ha ab
+        simp (config := {zeta := false}) at ha hb
+        have : b ≤ i'.succ := by obtain rfl | hb := hb <;> [rfl; exact Nat.le_succ_of_le (hT1 _ hb)]
+        have ha := ha.resolve_left <| ne_of_lt <| lt_of_lt_of_le ab this
+        obtain rfl | hb := hb
+        · exact hG1 i' _ le_rfl ic h1 _ ha ab
+        · exact hG2 _ (Nat.le_of_lt ic) h2 _ hb bc _ ha ab
+    · exact satisfies_noKHoleClausesCore T hh
+        (fun x hx => Nat.le_succ_of_le (hT1 _ hx))
+        (fun s sz hs' => hs _ sz fun x hx => Nat.le_of_lt (hs' _ hx))
+        (fun b c ib => hG1 _ _ (Nat.le_of_lt ib))
+        (fun c ic => hG2 _ (Nat.le_of_lt ic))
+  · simp at k0; simp [k0, hh] at hs
+termination_by _ => w.rlen - i
+decreasing_by decreasing_with omega
+
+theorem satisfies_naiveEncoding (w : CanonicalPoints) (k : Nat) :
+    ¬σHasEmptyKGon k w.toFinset →
+    (naiveEncoding k w.rlen).eval w.toPropAssn := by
+  simp [naiveEncoding, satisfies_baseEncoding, satisfies_signotopeClauses2,
+    satisfies_holeDefClauses0, noKHoleClauses]
+  intro noholes k0
+  have (s) (hs : s.card = k) : ¬isKHole w s := fun hn => by
+    refine noholes ⟨s.map ⟨(w[·]), fun i j => w.eq_iff'.1⟩, by simp [hs], ?_⟩
+    simp [Set.subset_def, w.mem_toFinset_iff, w.eq_iff']
+    intro a ha b hb c hc ab ac bc
+    have nd : Nodup [a, b, c] := by simp [*]
+    have : ∀ x ∈ [a, b, c], x ∈ s := by simp [*]
+    have ⟨l, lp, ls⟩ : ∃ l : List _, l.Perm [a, b, c] ∧ l.Sorted (· < ·) :=
+      ⟨[a,b,c].mergeSort (· ≤ ·), perm_mergeSort ..,
+        (sorted_mergeSort ..).imp₂ (fun _ _ => lt_of_le_of_ne) ((perm_mergeSort ..).nodup_iff.2 nd)⟩
+    have : ∀ x ∈ l, x ∈ s := fun x h => this _ (lp.subset h)
+    match l, lp.length_eq with | [a', b', c'], _ => ?_
+    simp at ls this
+    exact (σIsEmptyTriangleFor.perm (lp.map (w[·]))).1 <|
+      hn _ this.2.2 _ this.2.1 ls.2 _ this.1 ls.1.1
+  constructor
+  · apply satisfies_noKHoleClausesCore {0} ?_ (by simp) (fun s sz hs => this _ ?_)
+    · simp [isKHole1]
+    · simp [isKHole2, isKHole1]
+    · simp [isKHole, isKHole1, isKHole2]
+    · rw [← Finset.insert_eq, Finset.card_insert_of_not_mem, sz, Nat.sub_add_cancel k0]
+      exact fun h => lt_irrefl _ (hs _ h)
+  · apply satisfies_noKHoleClausesCore ∅ ?_ (by simp) (fun s hs => by simp [this _ hs])
+    · simp [isKHole1]
+    · simp [isKHole2, isKHole1]
+    · simp [isKHole]
+
+end CanonicalPoints
