Lean/Geo/Naive/Encoding.lean
@@ -1,0 +1,36 @@
+import Mathlib.Data.Fin.Basic
+import Mathlib.Data.List.Range
+import Geo.SAT.ToLeanSAT.EncodeProof
+import Geo.KGon.Var
+import Geo.KGon.Encoding
+
+namespace Geo
+
+open LeanSAT Var
+
+def noKHoleClausesCore (n k : Nat) (i : Nat)
+    (G1 : Fin n → Fin n → PropForm (Var n)) (G2 : Fin n → PropForm (Var n)) : PropForm (Var n) :=
+  if 0 < k then
+    .guard (i < n) fun hi =>
+    .and (.imp (G2 ⟨i, hi⟩) <|
+      noKHoleClausesCore n (k-1) (i+1)
+        (fun b c => .and (Var.hole ⟨i, hi⟩ b c) (G1 b c))
+        (fun c => .and (G1 ⟨i, hi⟩ c) (G2 c))) <|
+    noKHoleClausesCore n k (i+1) G1 G2
+  else
+    .false
+termination_by _ => n - i
+decreasing_by decreasing_with omega
+
+def noKHoleClauses (k n : Nat) : PropForm (Var n) :=
+  .guard (0 < k) fun _ =>
+    .and (noKHoleClausesCore n (k-1) 0 (fun b c => Var.hole₀ 0 b c) (fun _ => .true)) <|
+    noKHoleClausesCore n k 0 (fun _ _ => .true) (fun _ => .true)
+
+def naiveEncoding (k n : Nat) : PropForm (Var n) :=
+  .flatCNF <| .all #[baseEncoding n, signotopeClauses2 n, holeDefClauses0 n, noKHoleClauses k n]
+
+def naiveCNF (k rlen : Nat) : ICnf := (Geo.naiveEncoding k rlen |>.toICnf compare).2
+
+-- set_option profiler true in
+-- #eval let cnf := Geo.naiveCNF 10; (cnf.size, cnf.maxVar)
