Lean/Geo/RunEncoding.lean
@@ -1,0 +1,31 @@
+import Geo.Naive.Encoding
+import Geo.Hexagon.Encoding
+import LeanSAT.Solver.Dimacs
+
+open LeanSAT
+
+-- instance : Solver IO := Solver.Impl.DimacsCommand "cadical"
+
+def main (args : List String) : IO Unit := do
+  let help {α} : IO α := do
+    IO.println "\
+      usage: lake exe encode (gon|hole) <k> <n> [vars.out]\n\
+      where 3 <= k <= 6"
+    IO.Process.exit 1
+  let kind::k::n::rest := args | help
+  match kind with
+  | "gon" => IO.println "TODO: k-gon encoding unsupported"
+  | "hole" =>
+    let some k := String.toNat? k | help
+    let some n := String.toNat? n | help
+    let rlen + 1 := n | throw (.userError "n must be positive")
+    let (vars, enc) ← if k = 6 then
+      pure <| (Geo.hexagonEncoding rlen).toICnf compare
+    else
+      pure <| (Geo.naiveEncoding k rlen).toICnf compare
+    if let out::_ := rest then
+      let h ← IO.FS.Handle.mk out IO.FS.Mode.write
+      for v in vars do
+        h.putStrLn v.toCode
+    Solver.Dimacs.printFormula (IO.print) enc
+  | _ => help
