Lean/lakefile.lean
@@ -18,8 +18,5 @@ lean_lib «Geo» where
 lean_exe run_geo where
   root := `Geo
 
-lean_exe triangle where
-  root := `Geo.Triangle.RunEncoding
-
-lean_exe hexagon where
-  root := `Geo.Hexagon.RunEncoding
+lean_exe encode where
+  root := `Geo.RunEncoding
